prefix graph: <https://triplydb.com/Triply/value/graphs/>
prefix owl: <http://www.w3.org/2002/07/owl#>
prefix rdfs: <http://www.w3.org/2000/01/rdf-schema#>
prefix value: <https://triplydb.com/Triply/value/>
prefix void: <http://rdfs.org/ns/void#>

value:
  a void:Dataset;
  void:subset
    graph:vocab.

graph:vocab
  a owl:Ontology;
  rdfs:comment "A vocabulary for representing compound values, i.e., complex values that are composed out of one or more atomic values.  Such values are not supported by the current Linked Data standards."@en;
  rdfs:label "Triply Value Vocabulary"@en.

graph:vocab {
  # CLASSES

  value:AtomicValue
    rdfs:comment "The class of non-composed or atomic values, i.e., values that are composed or exactly one simple value."@en;
    rdfs:label "Atomic value"@en;
    rdfs:subClassOf value:Value.

  value:ClosedInterval
    rdfs:comment "The class of all closed intervals, i.e., intervals whose two simple values are neither minus infinity nor plus infinity."@en;
    rdfs:label "Closed interval"@en;
    rdfs:subClassOf value:Interval.

  value:CompoundValue
    rdfs:label "Compound value"@en;
    rdfs:subClassOf value:Value.

  value:Infinity
    rdfs:comment "The class of simple infinite values."@en;
    rdfs:label "Infinity"@en;
    rdfs:subClassOf value:AtomicValue.

  value:Interval
    rdfs:comment "The class of all interval values, i.e., complex values that are composed of examply two simple values.  The first value denotes the beginning of the interval; the second value denotes the end of the interval."@en;
    rdfs:label "Interval value"@en;
    rdfs:subClassOf value:CompoundValue.

  #value:LikertScale
  #  rdfs:comment "A scale consisting of 5 ordered values."@en;
  #  rdfs:label "Likert scale"@en;
  #  rdfs:subClassOf rdfs:Datatype.

  #value:LikertValue
  #  rdfs:comment "A value that belongs to a Likert scale."@en;
  #  rdfs:label "Likert value"@en;
  #  rdfs:subClassOf value:CompoundValue.

  value:OpenInterval
    rdfs:comment "The class of all open interval values, i.e., intervals where at least one of the simple values is (positive or negative) infinity."@en;
    rdfs:label "Open interval"@en;
    rdfs:subClassOf value:Interval.

  value:Value
    rdfs:comment "The generic class of all values, whether simple or complex."@en;
    rdfs:label "Value"@en;
    rdfs:subClassOf rdfs:Resource.

  # PROPERTIES

  value:lowerExclusive
    a owl:ObjectProperty;
    rdfs:comment "The lower exlcusive value of an interval."@en;
    rdfs:domain value:Interval;
    rdfs:label "Has lower exclusive value"@en;
    rdfs:range value:AtomicValue.

  value:lowerInclusive
    a owl:ObjectProperty;
    rdfs:comment "The lower exlcusive value of an interval."@en;
    rdfs:domain value:Interval;
    rdfs:label "Has lower inclusive value"@en;
    rdfs:range value:AtomicValue.

  value:higherExclusive
    a owl:ObjectProperty;
    rdfs:comment "The higher exclusive value of an interval."@en;
    rdfs:domain value:Interval;
    rdfs:label "Has higher exclusive value"@en;
    rdfs:range value:AtomicValue.

  value:higherInclusive
    a owl:ObjectProperty;
    rdfs:comment "The higher inclusive value of an interval."@en;
    rdfs:domain value:Interval;
    rdfs:label "Has higher inclusive value"@en;
    rdfs:range value:AtomicValue.

  #value:likertHighest
  #  a owl:ObjectProperty;
  #  rdfs:comment "The relationship between a Likert value type and its highest Likert value."@en;
  #  rdfs:domain value:LikertScale;
  #  rdfs:label "Has highest value"@en;
  #  rdfs:range value:LikertValue.

  #value:likertHigh
  #  a owl:ObjectProperty;
  #  rdfs:comment "The relationship between a Likert value type and its high (but not highest) Likert value."@en;
  #  rdfs:domain value:LikertScale;
  #  rdfs:label "Has high value"@en;
  #  rdfs:range value:LikertValue;
  #  value:lessThan value:likertHighest.

  #value:likertMiddle
  #  a owl:ObjectProperty;
  #  rdfs:comment "The relationship between a Likert value type and its middle Likert value."@en;
  #  rdfs:domain value:LikertScale;
  #  rdfs:label "Has middle value"@en;
  #  rdfs:range value:LikertValue;
  #  value:lessThan value:likertHigh.

  #value:likertLow
  #  a owl:ObjectProperty;
  #  rdfs:comment "The relationship between a Likert value type and its low (but not lowest) Likert value."@en;
  #  rdfs:domain value:LikertScale;
  #  rdfs:label "Has low value"@en;
  #  rdfs:range value:LikertValue;
  #  value:lessThan value:likertMiddle.

  #value:likertLowest
  #  a owl:ObjectProperty;
  #  rdfs:comment "The relationship between a Likert value type and its lowest Likert value."@en;
  #  rdfs:domain value:LikertScale;
  #  rdfs:label "Has lowest value"@en;
  #  rdfs:range value:LikertValue;
  #  value:lessThan value:likertLow.

  value:unit
    a owl:ObjectProperty;
    rdfs:comment "The relationship between a value and the unit of measure in which it is expressed."@en;
    rdfs:domain value:Value;
    rdfs:label "Has unit of measure"@en;
    rdfs:range rdfs:Datatype.

  # INSTANCES

  value:minusInfinity
    a value:Infinity;
    rdfs:label "Negative infinity"@en.

  value:infinity
    a value:Infinity;
    rdfs:label "Positive infinity"@en.
}
