prefix graph: <https://triplydb.com/Triply/value/graphs/>
prefix owl: <http://www.w3.org/2002/07/owl#>
prefix rdfs: <http://www.w3.org/2000/01/rdf-schema#>
prefix value: <https://triplydb.com/Triply/value/>
prefix void: <http://rdfs.org/ns/void#>

value:
  a void:Dataset;
  void:subset
    graph:vocab.

graph:vocab
  a owl:Ontology;
  rdfs:comment "A vocabulary for representing compound values, i.e., complex values that are composed out of one or more atomic values.  Such values are not supported by the current Linked Data standards."@en;
  rdfs:label "Triply Compound Value Vocabulary"@en.

graph:vocab {
  # Classes

  value:ClosedInterval
    rdfs:comment "The class of all closed intervals, i.e., intervals whose two simple values are neither minus infinity nor plus infinity."@en;
    rdfs:label "closed interval"@en;
    rdfs:subClassOf value:Interval.

  value:Infinity
    rdfs:comment "The class of simple infinite values."@en;
    rdfs:label "infinity"@en;
    rdfs:subClassOf value:Value.

  value:Interval
    rdfs:comment "The class of all interval values, i.e., complex values that are composed of examply two simple values.  The first value denotes the beginning of the interval; the second value denotes the end of the interval."@en;
    rdfs:label "interval value"@en;
    rdfs:subClassOf value:Value.

  value:OpenInterval
    rdfs:comment "The class of all open interval values, i.e., intervals where at least one of the simple values is (positive or negative) infinity."@en;
    rdfs:label "open interval"@en;
    rdfs:subClassOf value:Interval.

  value:Point
    rdfs:comment "The class of all point values, i.e., values that are composed or exactly one simple value."@en;
    rdfs:label "point value"@en;
    rdfs:subClassOf value:Value.

  value:Value
    rdfs:comment "The generic class of all values, whether simple or complex."@en;
    rdfs:label "value"@en;
    rdfs:subClassOf rdfs:Resource.

  # Properties

  value:lowerExclusive
    a owl:ObjectProperty;
    rdfs:comment "The lower exlcusive value of an interval."@en;
    rdfs:domain value:Interval;
    rdfs:label "has lower exclusive value"@en;
    rdfs:range value:Point.

  value:lowerInclusive
    a owl:ObjectProperty;
    rdfs:comment "The lower exlcusive value of an interval."@en;
    rdfs:domain value:Interval;
    rdfs:label "has lower exclusive value"@en;
    rdfs:range value:Point.

  value:higherExclusive
    a owl:ObjectProperty;
    rdfs:comment "The higher exclusive value of an interval."@en;
    rdfs:domain value:Interval;
    rdfs:label "has lower exclusive value"@en;
    rdfs:range value:Point.

  value:higherInclusive
    a owl:ObjectProperty;
    rdfs:comment "The higher inclusive value of an interval."@en;
    rdfs:domain value:Interval;
    rdfs:label "has lower exclusive value"@en;
    rdfs:range value:Point.

  value:unit
    a owl:ObjectProperty;
    rdfs:comment "The relationship between a value and the unit of measure in which it is expressed."@en;
    rdfs:domain value:Value;
    rdfs:label "has unit of measure"@en;
    rdfs:range rdfs:Datatype.

  # Instances

  value:minusInfinity
    a value:Infinity;
    rdfs:label "negative infinity"@en.

  value:infinity
    a value:Infinity;
    rdfs:label "positive infinity"@en.
}
